Move Get reasoning to byte_fs

src/Dafny/examples/fs/byte_fs.dfy
@@ -2,23 +2,103 @@ include "fs.dfy"
 
 module ByteFs {
   import opened Fs
+  import opened FsKinds
+  import opened JrnlSpec
   import opened Machine
+  import opened ByteSlice
 
   // TODO: implement this on top of the lower-level API in fs.dfy
 
-  function inode_data(sz: nat, blks: seq<Block>): (bs:seq<byte>)
-    requires forall i:nat | i < |blks| :: is_block(blks[i])
-    requires |blks| == Round.div_roundup_alt(sz, 4096)
-    ensures |bs| == sz
+  function inode_data_alt(d: InodeData): (bs:seq<byte>)
+    requires forall i:nat | i < |d.blks| :: is_block(d.blks[i])
+    requires |d.blks| == Round.div_roundup_alt(d.sz, 4096)
+    ensures |bs| == d.sz
   {
-    if sz % 4096 == 0 then (
+    var blks := d.blks;
+    if d.sz % 4096 == 0 then (
       C.concat_homogeneous_spec(blks, 4096);
       C.concat(blks)
       )
     else (
       C.concat_homogeneous_spec(C.without_last(blks), 4096);
       C.concat(C.without_last(blks)) +
-      C.last(blks)[..sz % 4096]
+      C.last(blks)[..d.sz % 4096]
       )
+  }
+
+  function inode_data(d: InodeData): (bs:seq<byte>)
+    requires forall i:nat | i < |d.blks| :: is_block(d.blks[i])
+    requires |d.blks| == Round.div_roundup_alt(d.sz, 4096)
+    ensures |bs| == d.sz
+  {
+    C.concat_homogeneous_spec(d.blks, 4096);
+    C.concat(d.blks)[..d.sz]
+  }
+
+  class ByteFilesys {
+    ghost var data: map<Ino, seq<byte>>;
+
+    const fs: Filesys;
+
+    function Repr(): set<object>
+    {
+      {this} + fs.Repr()
+    }
+
+    static predicate inode_blks_to_data(inode_blks: map<Ino, InodeData>, data: map<Ino, seq<byte>>)
+    {
+      && ino_dom(inode_blks)
+      && ino_dom(data)
+      && Valid_inode_blks(inode_blks)
+      && (forall ino | ino_ok(ino) :: data[ino] == inode_data(inode_blks[ino]))
+    }
+
+    predicate Valid()
+      reads this.Repr()
+    {
+      && fs.Valid()
+      && inode_blks_to_data(fs.inode_blks, data)
+    }
+
+    constructor Init(d: Disk)
+      ensures Valid()
+    {
+      fs := new Filesys.Init(d);
+      data := map ino | ino_ok(ino) :: [];
+    }
+
+    method Get(ino: Ino, off: uint64, len: uint64)
+      returns (bs: Bytes, ok: bool)
+      modifies {}
+      requires off % 4096 == 0 && len <= 4096
+      requires ino_ok(ino)
+      requires Valid() ensures Valid()
+      ensures ok ==>
+      && off as nat + len as nat <= |data[ino]|
+      && bs.data == data[ino][off..off+len]
+    {
+      var txn := fs.jrnl.Begin();
+      var i := fs.getInode(txn, ino);
+      if sum_overflows(off, len) || off+len > i.sz {
+        ok := false;
+        bs := NewBytes(0);
+        return;
+      }
+
+      ok := true;
+      if len == 0 {
+        bs := NewBytes(0);
+        return;
+      }
+      assert 0 < len <= 4096;
+
+      var blkoff: nat := off as nat / 4096;
+      bs := fs.getInodeBlk(txn, ino, i, blkoff);
+      C.concat_homogeneous_one_list(fs.inode_blks[ino].blks, blkoff, 4096);
+      bs.Subslice(0, len);
+      assert blkoff * 4096 == off as nat;
+
+      var _ := txn.Commit();
+    }
   }
 }
